examples/mw/MWC01proof.v
@@ -1,0 +1,189 @@
+Require Import HoareDef MWHeader MWC0 MWC1 SimModSem.
+Require Import Coqlib.
+Require Import ImpPrelude.
+Require Import Skeleton.
+Require Import PCM.
+Require Import ModSem Behavior.
+Require Import Relation_Definitions.
+Require Import Mem1.
+
+(*** TODO: export these in Coqlib or Universe ***)
+Require Import Relation_Operators.
+Require Import RelationPairs.
+From ITree Require Import
+     Events.MapDefault.
+From ExtLib Require Import
+     Core.RelDec
+     Structures.Maps
+     Data.Map.FMapAList.
+
+Require Import HTactics IPM ProofMode STB.
+
+Set Implicit Arguments.
+
+Local Open Scope nat_scope.
+
+
+
+Section PROOF.
+  Context `{Σ: GRA.t}.
+  
+  Lemma Own_unit
+    :
+      bi_entails True%I (Own ε)
+  .
+  Proof.
+    red. uipropall. ii. rr. esplits; et. rewrite URA.unit_idl. refl.
+  Qed.
+
+  Context `{@GRA.inG M Σ}.
+
+  Lemma embed_unit
+    :
+      (GRA.embed ε) = ε
+  .
+  Proof.
+    unfold GRA.embed.
+    Local Transparent GRA.to_URA. unfold GRA.to_URA. Local Opaque GRA.to_URA.
+    Local Transparent URA.unit. unfold URA.unit. Local Opaque URA.unit.
+    cbn.
+    apply func_ext_dep. i.
+    dependent destruction H. ss. rewrite inG_prf. cbn. des_ifs.
+  Qed.
+
+End PROOF.
+
+Section PROOF.
+  Context `{@GRA.inG M Σ}.
+
+  Lemma OwnM_unit
+    :
+      bi_entails True%I (OwnM ε)
+  .
+  Proof.
+    unfold OwnM. r. uipropall. ii. rr. esplits; et. rewrite embed_unit. rewrite URA.unit_idl. refl.
+  Qed.
+End PROOF.
+
+
+
+Section SIMMODSEM.
+
+  Context `{Σ: GRA.t}.
+  Context `{@GRA.inG memRA Σ}.
+
+  Let W: Type := Any.t * Any.t.
+
+  Variant sim_opt (opt: Z -> option val) (vs: list val): Prop :=
+  | sim_opt_intro
+      (SIM: ∀ k, 0 <= k < 100 -> opt k = List.nth_error vs (Z.to_nat k))
+  .
+
+  Let wf: _ -> W -> Prop :=
+    @mk_wf
+      _
+      unit
+      (* (fun _ _ mpr_tgt => (∃ (mr_tgt: AppRA), ⌜mpr_tgt = Any.pair tt↑ (GRA.embed mr_tgt)↑⌝ ** OwnM mr_tgt)%I) *)
+      (fun _ mp_src mp_tgt =>
+         (* (∃ lst0, ⌜mp_src = lst0↑⌝ ** (∃ blk vs, ⌜mp_tgt = (Vptr blk 0, lst0.(lst_map))↑⌝ ** OwnM ((blk,0%Z) |-> vs)) ∨ *)
+         (*                               (⌜mp_tgt = (Vnullptr, lst0.(lst_map))↑⌝))%I) *)
+
+
+         (* (∃ lst0 blk vs, ⌜mp_src = lst0↑⌝ ** ⌜mp_tgt = (Vptr blk 0, lst0.(lst_map))↑⌝ ** OwnM ((blk,0%Z) |-> vs) ** *)
+         (*                                      ⌜sim_opt lst0.(lst_opt) vs ∧ (lst0.(lst_map) = Vnullptr ∨ length vs = 100)⌝)%I) *)
+         (∃ lst0 blk vs, ⌜mp_src = lst0↑⌝ ** ⌜mp_tgt = (Vptr blk 0, lst0.(lst_map))↑⌝ **
+                                              (OwnM ((blk,0%Z) |-> vs) ** ⌜sim_opt lst0.(lst_opt) vs⌝ ** ⌜length vs = 100⌝) ∨
+                                              (⌜lst0.(lst_map) = Vnullptr⌝))%I)
+  .
+
+  Lemma points_to_nil
+        loc
+    :
+      <<EQ: loc |-> [] = ε>>
+  .
+  Proof.
+    unfold points_to. r. rewrite unfold_points_to. des_ifs. ss.
+    Local Transparent URA.unit. unfold URA.unit. ss. Local Opaque URA.unit.
+    unfold Auth.white. f_equal. apply func_ext; i. apply func_ext; i. des_ifs.
+    bsimpl; des; des_sumbool. clarify. lia.
+  Qed.
+
+  Opaque memRA.
+  Opaque mwRA.
+  Opaque Z.eq_dec Z.eqb.
+
+  Theorem correct: refines2 [MWC0.MW] [MWC1.MW].
+  Proof.
+    eapply adequacy_local2. econs; ss.
+    i. econstructor 1 with (wf:=wf) (le:=top2); et; swap 2 3.
+    { ss. }
+    { destruct (SkEnv.id2blk (Sk.load_skenv sk) "arr") eqn:T; cycle 1.
+      { exfalso. Local Transparent Sk.load_skenv. unfold Sk.load_skenv in *. Local Opaque Sk.load_skenv.
+        ss. uo. des_ifs. admit "ez". }
+      esplits. econs; ss. eapply to_semantic. iIntros "H". rewrite T. cbn. iSplits; ss. iRight; ss.
+    }
+
+    econs; ss.
+    { init. harg. mDesAll. des; clarify. des_u. steps. unfold mainF, MWC0.mainF. steps.
+      unfold ncall. steps. force_l. exists true. steps. force_l. eexists. steps. unfold ccallU. steps.
+      force_l; stb_tac; ss; clarify. steps.
+      hcall _ _ _ with "*".
+      { iModIntro. iSplits; ss; et.
+        { iPureIntro. instantiate (1:=100). cbn. refl. }
+        { ss. }
+      }
+      { esplits; ss; et.
+      mDesOr "A".
+      -
+      steps. unfold initF, ASSUME, GUARANTEE. steps.
+      force_r. exists Init. steps. force_r; ss. steps. force_r. eexists. steps. force_r; ss.
+      { esplits; et. admit "ez". }
+      steps. rename c0 into rm. rename c1 into ro. rename c into rf1.
+      rewrite URA.unit_id in _GUARANTEE0.
+      mCombine "A1" "A2". mEval ltac:(erewrite URA.add_comm; erewrite <- _GUARANTEE0) in "A1".
+      unfold ccallU. steps. des. clear_tac. mDesOwn "A1" as "B" "C".
+      hcall _ (_, _, _) _ with "A B".
+      { iModIntro. iDestruct "B" as "[B C]". iFrame. iSplits; ss; et. }
+      { esplits; ss; et. rr; ss. }
+      steps. mDesAll; clarify.
+      rewrite _UNWRAPU. steps. force_r. exists ε. steps. force_r; ss. steps. force_r. rename a into rm0.
+      eexists. steps. force_r; ss.
+      { rewrite URA.unit_id. esplits; et. admit "ez". }
+      steps. des; clarify.
+      mAssert _ with "C A".
+      { iCombine "A" "C" as "A". (* sym in _GUARANTEE. iRewrite _GUARANTEE in "A". *) iExact "A". }
+      mEval ltac:(erewrite <- _GUARANTEE) in "A1".
+
+      hret _; ss.
+      { iModIntro. iDestruct "A1" as "[[A B] C]". iFrame. iSplitL "A"; et. }
+    }
+
+    econs; ss.
+    { init. harg. mDesAll. des; clarify. rename x into mwf. rename a into _lower_layer_rm.
+      steps. unfold runF, ASSUME, GUARANTEE. steps.
+      force_r. exists Run. steps. force_r; ss. steps. force_r. eexists. steps. force_r; ss.
+      { esplits; et. admit "ez". }
+      steps. rename c0 into rm. rename c1 into ro. rename c into rf1.
+      rewrite URA.unit_id in _GUARANTEE0.
+      mCombine "A1" "A2". mEval ltac:(erewrite URA.add_comm; erewrite <- _GUARANTEE0) in "A1".
+      unfold ccallU. steps. des. clear_tac. mDesOwn "A1" as "B" "C".
+      hcall _ (_, _, _) _ with "A B".
+      { iModIntro. iDestruct "B" as "[B C]". iFrame. iSplits; ss; et. }
+      { esplits; ss; et. rr; ss. }
+      steps. mDesAll; clarify.
+      rewrite _UNWRAPU. steps. rewrite Any.upcast_downcast in *. clarify. steps.
+      force_r. exists ε. steps. force_r; ss. steps. force_r. rename a into rm0.
+      eexists. steps. force_r; ss.
+      { rewrite URA.unit_id. esplits; et. admit "ez". }
+      steps. des; clarify.
+      mAssert _ with "C A".
+      { iCombine "A" "C" as "A". (* sym in _GUARANTEE. iRewrite _GUARANTEE in "A". *) iExact "A". }
+      mEval ltac:(erewrite <- _GUARANTEE) in "A2".
+
+      hret _; ss.
+      { iModIntro. iDestruct "A2" as "[[A B] C]". iFrame. iSplitL "A"; et. }
+    }
+  Unshelve. all: ss. all: try exact 0.
+  Qed.
+
+End SIMMODSEM.
