examples/mw/MWC1.v
@@ -1,0 +1,118 @@
+Require Import Coqlib.
+Require Import ITreelib.
+Require Import ImpPrelude.
+Require Import STS.
+Require Import Behavior.
+Require Import ModSem.
+Require Import Skeleton.
+Require Import PCM.
+Require Import HoareDef.
+Require Import MWHeader.
+Require Import Mem1.
+
+Set Implicit Arguments.
+
+
+
+Section PROOF.
+
+  Notation pget := (p0 <- trigger PGet;; p0 <- p0↓ǃ;; Ret p0) (only parsing).
+  Notation pput p0 := (trigger (PPut p0↑)) (only parsing).
+
+  Record local_state: Type := mk_lst {
+    lst_dom: Z -> option unit;
+    lst_opt: Z -> option val;
+    lst_map: val;
+    (* lst_wf: forall k, (is_some (lst_opt k)) -> (is_some (lst_dom k)) *)
+  }
+  .
+
+  Notation upd_dom f := (lst0 <- pget;; pput (mk_lst (f lst0.(lst_dom)) lst0.(lst_opt) lst0.(lst_map))).
+  Notation upd_opt f := (lst0 <- pget;; pput (mk_lst lst0.(lst_dom) (f lst0.(lst_opt)) lst0.(lst_map))).
+  Notation upd_map f := (lst0 <- pget;; pput (mk_lst lst0.(lst_dom) lst0.(lst_opt) (f lst0.(lst_map)))).
+
+  Let Es := (hAPCE +' Es).
+
+  Definition ncall X Y (f: string): itree Es Y :=
+    `b: bool <- trigger (Choose bool);;
+    if b
+    then `x: X <- trigger (Choose _);; ccallU f x
+    else r <- trigger (Choose _);; Ret r
+  .
+
+  Definition loopF: list val -> itree Es val :=
+    fun varg =>
+      _ <- (pargs [] varg)?;;
+      `_: val <- ccallU "run" ([]: list val);;
+      `_: val <- ccallU "loop" ([]: list val);;
+      Ret Vundef
+  .
+
+  Definition mainF: list val -> itree Es val :=
+    fun varg =>
+      _ <- (pargs [] varg)?;;
+      ncall (list val) val "alloc";;;
+      `map: val <- ccallU "new" ([]: list val);;
+      upd_map (fun _ => map);;;
+      `_: val <- ccallU "loop" ([]: list val);;
+      Ret Vundef
+  .
+
+  Definition putF: list val -> itree Es val :=
+    fun varg =>
+      '(k, v) <- (pargs [Tint; Tuntyped] varg)?;;
+      lst0 <- pget;; 
+      assume(lst0.(lst_map) <> Vnullptr);;;
+      assume((0 <= k)%Z);;;
+      b <- trigger (Choose _);;
+      (if (b: bool)
+       then ncall (list val) val "store";;; upd_opt (fun opt => add k v opt)
+       else `_: val <- ccallU "update" ([lst0.(lst_map); Vint k; v]);; upd_dom (fun dom => add k tt dom));;;
+      trigger (Syscall "print" [Vint k]↑ top1);;;
+      trigger (Syscall "print" [v]↑ top1);;;
+      Ret Vundef
+  .
+
+  Definition getF: list val -> itree Es val :=
+    fun varg =>
+      k <- (pargs [Tint] varg)?;;
+      `lst0: local_state <- pget;;
+      assume(lst0.(lst_map) <> Vnullptr);;;
+      assume(is_some (lst0.(lst_dom) k) \/ is_some (lst0.(lst_opt) k));;;
+      v <- (match lst0.(lst_opt) k with
+            | Some v => ncall (list val) val "load";;; Ret v
+            | _ => ccallU "access" ([lst0.(lst_map); Vint k])
+            end);;
+      trigger (Syscall "print" [Vint k]↑ top1);;; (*** TODO: make something like "syscallu" ***)
+      trigger (Syscall "print" [v]↑ top1);;;
+      Ret Vundef
+  .
+
+  Context `{Σ: GRA.t}.
+
+  Definition MWsbtb: list (string * fspecbody) :=
+    [("main", mk_specbody fspec_trivial (cfunU mainF));
+    ("loop", mk_specbody fspec_trivial (cfunU loopF));
+    ("put", mk_specbody fspec_trivial (cfunU putF));
+    ("get", mk_specbody fspec_trivial (cfunU getF))
+    ].
+
+  Definition SMWSem: SModSem.t := {|
+    SModSem.fnsems := MWsbtb;
+    SModSem.mn := "MW";
+    SModSem.initial_mr := ε;
+    SModSem.initial_st := (mk_lst empty empty Vnullptr)↑;
+  |}
+  .
+
+  Definition SMW: SMod.t := {|
+    SMod.get_modsem := fun _ => SMWSem;
+    SMod.sk := [("main", Sk.Gfun); ("loop", Sk.Gfun); ("put", Sk.Gfun); ("get", Sk.Gfun)];
+  |}
+  .
+
+  Context `{@GRA.inG memRA Σ}.
+
+  Definition MW: Mod.t := (SMod.to_tgt (fun _ => GlobalStbC)) SMW.
+
+End PROOF.
